Test/tutorial/ImpVerifiedCompiler/Semantics.dfy
@@ -2,6 +2,10 @@ least predicate star<T(!new)>(R: (T,T) -> bool, conf1: T, conf2: T) {
 	(conf1 == conf2) || (exists conf_inter: T :: R(conf1, conf_inter) && star(R,conf_inter, conf2))
 }
 
+least predicate plus<T(!new)>(R: (T,T) -> bool, conf1: T, conf2: T) {
+	(exists conf_inter: T :: R(conf1, conf_inter) && star(R,conf_inter, conf2))
+}
+
 predicate all_seq_inf<T(!new)>(R: (T,T) -> bool,conf: T) {
 	forall conf2: T :: star(R,conf,conf2) ==> exists conf3: T :: R(conf2,conf3)
 }
