Test/tutorial/ImpVerifiedCompiler/SimulationRelationCont.dfy
@@ -1,3 +1,37 @@
 include "SimulationRelation.dfy"
 include "ImpReductionContSem.dfy"
+include "Mach.dfy"
+include "MachSemantics.dfy"
+include "Compiler.dfy"
 
+least predicate compile_cont(C: code, k: cont, pc: nat) {
+	if ! (pc < |C|) then false else
+	match (k,C[pc]) {
+		case (Kstop,Ihalt) => true
+		case (Kseq(c,k),_) =>
+			var pc' := pc + |compile_com(c)|;
+			&& code_at(C, pc, (compile_com(c)))
+			&& compile_cont(C, k, pc')
+		case (Kwhile(b,c,k),Ibranch(ofs)) =>
+			var pc' := pc + 1 + ofs;
+			var pc'' := pc' + |compile_com(CWhile(b, c))|;
+			&& pc' > 0
+			&& pc'' > 0	
+      && code_at(C, pc', (compile_com(CWhile(b, c)))) 
+      && compile_cont(C, k, pc'')
+		case (_,Ibranch(ofs)) =>
+			var pc' := pc + 1 + ofs;
+			&& pc' > 0
+      && compile_cont(C, k, pc')
+		case _ => false
+	}
+	
+}
+
+predicate match_config(C: code, hl: conf, ll:configuration) {
+	var (c,k,s) := hl;
+	var (pc,stk,str) := ll;
+	&& code_at(C, pc, (compile_com(c)))
+	&&  compile_cont(C, k, (pc + |compile_com(c)|))
+	&& stk == [] 
+}
