Test/tutorial/ImpVerifiedCompiler/Proof.dfy
@@ -1,0 +1,49 @@
+include "SimulationRelationCont.dfy"
+include "ImpReductionContSem.dfy"
+include "MachSemantics.dfy"	
+include "SemanticsProperties.dfy"	
+
+predicate Star<T(!new)>(R: (T,T) -> bool, conf1: T, conf2: T) {
+  star(R, conf1, conf2)
+}
+
+lemma simulation_step(C: code, impconf1: conf, impconf2: conf, machconf1: configuration)
+	requires step(impconf1,impconf2)
+	requires match_config(C, impconf1, machconf1)
+	ensures exists machconf2: configuration :: star((c1,c2) => transition(C,c1,c2),machconf1,machconf2) && match_config(C, impconf2, machconf2) 
+
+least lemma simulation_steps(C: code, impconf1: conf, impconf2: conf, machconf1: configuration)
+	requires star(step,impconf1,impconf2)
+	requires match_config(C, impconf1, machconf1)
+	ensures exists machconf2: configuration :: star((c1,c2) => transition(C,c1,c2),machconf1,machconf2) && match_config(C, impconf2, machconf2)
+{
+	var tr := (c1,c2) => transition(C,c1,c2);
+	if impconf1 == impconf2 {
+	} else {
+		var impconf_inter :| step(impconf1, impconf_inter) && star(step,impconf_inter, impconf2);
+		simulation_step(C,impconf1,impconf_inter,machconf1);
+		var machconf_inter :| Star(tr,machconf1,machconf_inter) && match_config(C, impconf_inter, machconf_inter);
+		simulation_steps(C, impconf_inter, impconf2, machconf_inter);
+		// I do not know why the skolemization needs this assert
+		// It might have to do with the lambda
+		assert exists machconf2: configuration :: Star((c1,c2) => transition(C,c1,c2),machconf_inter,machconf2) && match_config(C, impconf2, machconf2);
+		var machconf2 :| Star((c1,c2) => transition(C,c1,c2),machconf_inter,machconf2) && match_config(C, impconf2, machconf2);
+		
+		star_trans_sequent<configuration>(tr,machconf1,machconf_inter,machconf2);
+	}
+}
+	
+lemma match_initial_configs(c: com, s: store)
+	ensures match_config((compile_program(c)), (c, Kstop, s), (0, [], s))
+{
+	var C := compile_program(c);
+	assert code_at(C, 0, compile_com(c)) by {
+		var C1: code := [];
+		var C3 := [Ihalt];
+		assert C == C1 + compile_com(c) + C3;
+	}
+	assert C[|compile_com(c)|] == Ihalt;
+	assert compile_cont(C, Kstop, |compile_com(c)|);
+}
+
+
